More reorganization.

PropositionalLogic/Semantics/Kripke.v
@@ -4,160 +4,73 @@ Require Import Coq.Relations.Relation_Definitions.
 Require Import Logic.GeneralLogic.Base.
 Require Import Logic.MinimunLogic.Syntax.
 Require Import Logic.PropositionalLogic.Syntax.
+Require Import Logic.PropositionalLogic.KripkeModel.
 
 Local Open Scope logic_base.
 Local Open Scope syntax.
 Local Open Scope kripke_model.
 Import PropositionalLanguageNotation.
 Import KripkeModelFamilyNotation.
-
-Class KripkeIntuitionisticModel (worlds: Type): Type := {
-  Korder: worlds -> worlds -> Prop; (* <= *)
-  Korder_PreOrder:> PreOrder Korder
-}.
-
-Module KripkeModelNotation_Intuitionistic.
-
-Infix "<=" := Korder: kripke_model.
-
-End KripkeModelNotation_Intuitionistic.
-
 Import KripkeModelNotation_Intuitionistic.
 
-Class IdentityKripkeIntuitionisticModel (worlds: Type) {kiW: KripkeIntuitionisticModel worlds} : Prop := {
-  Korder_identity: forall m n: worlds, m <= n -> m = n
+Module Semantics.
+
+Definition impp {worlds: Type} {R: Relation worlds} (X: Ensemble worlds) (Y: Ensemble worlds): Ensemble worlds :=
+  fun m => forall n, m <= n -> X n -> Y n.
+
+Definition andp {worlds: Type} (X: Ensemble worlds) (Y: Ensemble worlds): Ensemble worlds :=
+  fun m => X m /\ Y m.
+
+Definition orp {worlds: Type} (X: Ensemble worlds) (Y: Ensemble worlds): Ensemble worlds :=
+  fun m => X m \/ Y m.
+
+Definition falsep {worlds: Type}: Ensemble worlds := fun m => False.
+
+End Semantics.
+
+Class KripkeIntuitionisticSemantics (L: Language) {nL: NormalLanguage L} {pL: PropositionalLanguage L} (MD: Model) {kMD: KripkeModel MD} (M: Kmodel) {R: Relation (Kworlds M)} {kiM: KripkeIntuitionisticModel (Kworlds M)} (SM: Semantics L MD) : Type := {
+  denote_closed: forall x, upwards_closed_Kdenote (Kdenotation M x);
+  denote_impp: forall x y, Same_set _ (Kdenotation M (x --> y)) (Semantics.impp (Kdenotation M x) (Kdenotation M y));
+  denote_andp: forall x y, Same_set _ (Kdenotation M (x && y)) (Semantics.andp (Kdenotation M x) (Kdenotation M y));
+  denote_orp: forall x y, Same_set _ (Kdenotation M (x || y)) (Semantics.orp (Kdenotation M x) (Kdenotation M y));
+  denote_falsep: Same_set _ (Kdenotation M FF) Semantics.falsep
 }.
 
-Class NoBranchKripkeIntuitionisticModel (worlds: Type) {kiW: KripkeIntuitionisticModel worlds} : Prop := {
-  Korder_no_branch: forall m1 m2 n: worlds, n <= m1 -> n <= m2 -> m1 <= m2 \/ m2 <= m1
-}.
-
-Class BranchJoinKripkeIntuitionisticModel (worlds: Type) {kiW: KripkeIntuitionisticModel worlds} : Prop := {
-  Korder_branch_join: forall m1 m2 n: worlds, n <= m1 -> n <= m2 -> exists m, m1 <= m /\ m2 <= m
-}.
-
-Definition Korder_stable {worlds: Type} {kiW: KripkeIntuitionisticModel worlds} (P: worlds -> Prop): Prop :=
-  forall w1 w2, w1 <= w2 -> (P w1 <-> P w2).
-
-Class KripkeIntuitionisticSemantics (L: Language) {nL: NormalLanguage L} {pL: PropositionalLanguage L} (MD: Model) {kMD: KripkeModel MD} (M: Kmodel) {kiW: KripkeIntuitionisticModel (Kworlds M)} (SM: Semantics L MD) : Type := {
-  sat_mono: forall m n x, m <= n -> KRIPKE: M , m |= x -> KRIPKE: M , n |= x;
-  sat_impp: forall m x y, KRIPKE: M , m |= x --> y <-> (forall n, m <= n -> KRIPKE: M , n |= x -> KRIPKE: M , n |= y);
-  sat_andp: forall m x y, KRIPKE: M , m |= x && y <-> (KRIPKE: M , m |= x /\ KRIPKE: M , m |= y);
-  sat_orp: forall m x y, KRIPKE: M , m |= x || y <-> (KRIPKE: M , m |= x \/ KRIPKE: M , m |= y);
-  sat_falsep: forall m, ~ KRIPKE: M , m |= FF
-}.
-
-Module KripkeSemantics.
-
-Import PropositionalLanguage.
-
-Record frame: Type := {
-  underlying_set:> Type;
-  Korder: relation underlying_set; (* <= *)
-  Korder_preorder: PreOrder Korder
-}.
-
-Infix "<=" := (Korder _): TheKripkeSemantics.
-
-Local Open Scope TheKripkeSemantics.
-
-Definition sem (f: frame) := sig (fun s: Ensemble f => forall x y, x <= y -> s x -> s y).
-
-Program Definition sem_and {F: frame} (X: sem F) (Y: sem F): sem F :=
-  fun x: F => X x /\ Y x.
-Next Obligation.
-  split.
-  + eapply (proj2_sig X); eauto.
-  + eapply (proj2_sig Y); eauto.
-Qed.
-
-Program Definition sem_or {F: frame} (X: sem F) (Y: sem F): sem F :=
-  fun x: F => X x \/ Y x.
-Next Obligation.
-  destruct H0; [left | right].
-  + eapply (proj2_sig X); eauto.
-  + eapply (proj2_sig Y); eauto.
-Qed.
-
-Program Definition sem_imp {F: frame} (X: sem F) (Y: sem F): sem F :=
-  fun x: F =>
-    forall y: F, x <= y -> X y -> Y y.
-Next Obligation.
-  revert H2; apply H0.
-  pose proof @PreOrder_Transitive _ _ (Korder_preorder F).
-  transitivity y; auto.
-Qed.
-
-Program Definition sem_true {F: frame}: sem F :=
-  fun x: F => True.
-
-Program Definition sem_false {F: frame}: sem F :=
-  fun x: F => False.
-
-Definition sem_neg {F: frame} (X: sem F): sem F :=
-  sem_imp X sem_false.
-
-Definition sem_iff {F: frame} (X: sem F) (Y: sem F): sem F :=
-  sem_and (sem_imp X Y) (sem_imp Y X).
-
-Definition denotation {Var: Type} (F: frame) (eval: Var -> sem F): expr Var -> sem F :=
-  fix denotation (x: expr Var): sem F:=
-  match x with
-  | andp y z => sem_and (denotation y) (denotation z)
-  | orp y z => sem_or (denotation y) (denotation z)
-  | impp y z => sem_imp (denotation y) (denotation z)
-  | falsep => sem_false
-  | varp p => eval p
-  end.
-
-Section KripkeSemantics.
-Context (Var: Type).
-
-Record Kmodel : Type := {
-  underlying_frame :> frame;
-  Kvar: Var -> sem underlying_frame
-}.
-
-Record model: Type := {
-  underlying_model :> Kmodel;
-  elm: underlying_model
-}.
-
-Instance L: Language := PropositionalLanguage.L Var.
-Instance MD: Model := Build_Model model.
-
-Instance kMD: KripkeModel MD :=
-  Build_KripkeModel _
-    Kmodel
-    (fun M => M)
-    (fun M m => Build_model M m).
-
-Instance kiM (M: Kmodel): KripkeIntuitionisticModel (Kworlds M) :=
-  Build_KripkeIntuitionisticModel (Kworlds M) (Korder M) (Korder_preorder _).
-
-Instance SM: Semantics L MD :=
-  Build_Semantics L MD
-   (fun M x => proj1_sig (denotation M (Kvar M) x) (elm M)).
-
-Instance kiSM (M: Kmodel): KripkeIntuitionisticSemantics L MD M SM.
+Lemma sat_mono {L: Language} {nL: NormalLanguage L} {pL: PropositionalLanguage L} {MD: Model} {kMD: KripkeModel MD} {M: Kmodel} {R: Relation (Kworlds M)} {kiM: KripkeIntuitionisticModel (Kworlds M)} {SM: Semantics L MD} {kSM: KripkeIntuitionisticSemantics L MD M SM}: forall m n x, m <= n -> KRIPKE: M , m |= x -> KRIPKE: M , n |= x.
 Proof.
-  apply Build_KripkeIntuitionisticSemantics.
-  + hnf; simpl; intros.
-    eapply (proj2_sig (denotation M (Kvar M) x)); eauto.
-  + split; auto.
-  + split; auto.
-  + split; auto.
-  + intros; simpl. auto.
-Defined.
+  intros ? ? ? ?.
+  unfold satisfies.
+  apply (denote_closed x); auto.
+Qed.
 
-Definition Kmodel_Identity: Kmodel -> Prop := fun M =>
-  IdentityKripkeIntuitionisticModel (Kworlds M).
+Lemma sat_impp {L: Language} {nL: NormalLanguage L} {pL: PropositionalLanguage L} {MD: Model} {kMD: KripkeModel MD} {M: Kmodel} {R: Relation (Kworlds M)} {kiM: KripkeIntuitionisticModel (Kworlds M)} {SM: Semantics L MD} {kSM: KripkeIntuitionisticSemantics L MD M SM}: forall m x y, KRIPKE: M , m |= x --> y <-> (forall n, m <= n -> KRIPKE: M , n |= x -> KRIPKE: M , n |= y).
+Proof.
+  intros; simpl.
+  unfold satisfies.
+  destruct (denote_impp x y).
+  split; [apply H | apply H0].
+Qed.
 
-Definition Kmodel_NoBranch: Kmodel -> Prop := fun M =>
-  NoBranchKripkeIntuitionisticModel (Kworlds M).
+Lemma sat_andp {L: Language} {nL: NormalLanguage L} {pL: PropositionalLanguage L} {MD: Model} {kMD: KripkeModel MD} {M: Kmodel} {R: Relation (Kworlds M)} {kiM: KripkeIntuitionisticModel (Kworlds M)} {SM: Semantics L MD} {kSM: KripkeIntuitionisticSemantics L MD M SM}: forall m x y, KRIPKE: M , m |= x && y <-> (KRIPKE: M , m |= x /\ KRIPKE: M , m |= y).
+Proof.
+  intros; simpl.
+  unfold satisfies.
+  destruct (denote_andp x y).
+  split; [apply H | apply H0].
+Qed.
 
-Definition Kmodel_BranchJoin: Kmodel -> Prop := fun M =>
-  BranchJoinKripkeIntuitionisticModel (Kworlds M).
+Lemma sat_orp {L: Language} {nL: NormalLanguage L} {pL: PropositionalLanguage L} {MD: Model} {kMD: KripkeModel MD} {M: Kmodel} {R: Relation (Kworlds M)} {kiM: KripkeIntuitionisticModel (Kworlds M)} {SM: Semantics L MD} {kSM: KripkeIntuitionisticSemantics L MD M SM}: forall m x y, KRIPKE: M , m |= x || y <-> (KRIPKE: M , m |= x \/ KRIPKE: M , m |= y).
+Proof.
+  intros; simpl.
+  unfold satisfies.
+  destruct (denote_orp x y).
+  split; [apply H | apply H0].
+Qed.
 
-End KripkeSemantics.
-End KripkeSemantics.
+Lemma sat_falsep {L: Language} {nL: NormalLanguage L} {pL: PropositionalLanguage L} {MD: Model} {kMD: KripkeModel MD} {M: Kmodel} {R: Relation (Kworlds M)} {kiM: KripkeIntuitionisticModel (Kworlds M)} {SM: Semantics L MD} {kSM: KripkeIntuitionisticSemantics L MD M SM}: forall m, KRIPKE: M , m |= FF <-> False.
+Proof.
+  intros; simpl.
+  unfold satisfies.
+  destruct denote_falsep.
+  split; [apply H | apply H0].
+Qed.
