PropositionalLogic/DeepEmbeddedInstance/KripkeSemantics.v
@@ -1,0 +1,124 @@
+Require Import Coq.Logic.Classical_Prop.
+Require Import Coq.Classes.RelationClasses.
+Require Import Coq.Relations.Relation_Definitions.
+Require Import Logic.lib.Ensembles_ext.
+Require Import Logic.GeneralLogic.Base.
+Require Import Logic.MinimunLogic.Syntax.
+Require Import Logic.PropositionalLogic.Syntax.
+Require Import Logic.PropositionalLogic.Semantics.Kripke.
+Require Import Logic.PropositionalLogic.DeepEmbeddedInstance.PropositionalLanguage.
+
+Module KripkeSemantics.
+
+Import PropositionalLanguage.
+
+Record frame: Type := {
+  underlying_set:> Type;
+  Krelation: relation underlying_set; (* <= *)
+  Krelation_Preorder: PreOrder Krelation
+}.
+
+Infix "<=" := (Krelation _): TheKripkeSemantics.
+
+Local Open Scope TheKripkeSemantics.
+
+Definition sem (f: frame) := sig (fun s: Ensemble f => forall x y, x <= y -> s x -> s y).
+
+Program Definition sem_and {F: frame} (X: sem F) (Y: sem F): sem F := Semantics.andp X Y.
+Next Obligation.
+  destruct H0.
+  split.
+  + eapply (proj2_sig X); eauto.
+  + eapply (proj2_sig Y); eauto.
+Qed.
+
+Program Definition sem_or {F: frame} (X: sem F) (Y: sem F): sem F :=
+  fun x: F => X x \/ Y x.
+Next Obligation.
+  destruct H0; [left | right].
+  + eapply (proj2_sig X); eauto.
+  + eapply (proj2_sig Y); eauto.
+Qed.
+
+Program Definition sem_imp {F: frame} (X: sem F) (Y: sem F): sem F :=
+  fun x: F =>
+    forall y: F, x <= y -> X y -> Y y.
+Next Obligation.
+  revert H2; apply H0.
+  pose proof @PreOrder_Transitive _ _ (Korder_preorder F).
+  transitivity y; auto.
+Qed.
+
+Program Definition sem_true {F: frame}: sem F :=
+  fun x: F => True.
+
+Program Definition sem_false {F: frame}: sem F :=
+  fun x: F => False.
+
+Definition sem_neg {F: frame} (X: sem F): sem F :=
+  sem_imp X sem_false.
+
+Definition sem_iff {F: frame} (X: sem F) (Y: sem F): sem F :=
+  sem_and (sem_imp X Y) (sem_imp Y X).
+
+Definition denotation {Var: Type} (F: frame) (eval: Var -> sem F): expr Var -> sem F :=
+  fix denotation (x: expr Var): sem F:=
+  match x with
+  | andp y z => sem_and (denotation y) (denotation z)
+  | orp y z => sem_or (denotation y) (denotation z)
+  | impp y z => sem_imp (denotation y) (denotation z)
+  | falsep => sem_false
+  | varp p => eval p
+  end.
+
+Section KripkeSemantics.
+Context (Var: Type).
+
+Record Kmodel : Type := {
+  underlying_frame :> frame;
+  Kvar: Var -> sem underlying_frame
+}.
+
+Record model: Type := {
+  underlying_model :> Kmodel;
+  elm: underlying_model
+}.
+
+Instance L: Language := PropositionalLanguage.L Var.
+Instance MD: Model := Build_Model model.
+
+Instance kMD: KripkeModel MD :=
+  Build_KripkeModel _
+    Kmodel
+    (fun M => M)
+    (fun M m => Build_model M m).
+
+Instance kiM (M: Kmodel): KripkeIntuitionisticModel (Kworlds M) :=
+  Build_KripkeIntuitionisticModel (Kworlds M) (Korder M) (Korder_preorder _).
+
+Instance SM: Semantics L MD :=
+  Build_Semantics L MD
+   (fun M x => proj1_sig (denotation M (Kvar M) x) (elm M)).
+
+Instance kiSM (M: Kmodel): KripkeIntuitionisticSemantics L MD M SM.
+Proof.
+  apply Build_KripkeIntuitionisticSemantics.
+  + hnf; simpl; intros.
+    eapply (proj2_sig (denotation M (Kvar M) x)); eauto.
+  + split; auto.
+  + split; auto.
+  + split; auto.
+  + intros; simpl. auto.
+Defined.
+
+Definition Kmodel_Identity: Kmodel -> Prop := fun M =>
+  IdentityKripkeIntuitionisticModel (Kworlds M).
+
+Definition Kmodel_NoBranch: Kmodel -> Prop := fun M =>
+  NoBranchKripkeIntuitionisticModel (Kworlds M).
+
+Definition Kmodel_BranchJoin: Kmodel -> Prop := fun M =>
+  BranchJoinKripkeIntuitionisticModel (Kworlds M).
+
+End KripkeSemantics.
+End KripkeSemantics.
