PropositionalLogic/KripkeModel.v
@@ -1,0 +1,39 @@
+Require Import Coq.Sets.Ensembles.
+Require Import Coq.Logic.Classical_Prop.
+Require Import Coq.Classes.RelationClasses.
+Require Import Coq.Relations.Relation_Definitions.
+
+Class Relation (worlds: Type): Type :=
+  Krelation: worlds -> worlds -> Prop (* <= *).
+
+Class KripkeIntuitionisticModel (worlds: Type) {R: Relation worlds}: Type :=
+  Krelation_Preorder :> PreOrder Krelation.
+
+Module KripkeModelNotation_Intuitionistic.
+
+Infix "<=" := Krelation: kripke_model.
+
+End KripkeModelNotation_Intuitionistic.
+
+Import KripkeModelNotation_Intuitionistic.
+
+Local Open Scope kripke_model.
+
+Definition upwards_closed_Kdenote {worlds: Type} {R: Relation worlds} (d: Ensemble worlds): Prop :=
+  forall n m, n <= m -> d n -> d m.
+
+Definition Krelation_stable_Kdenote {worlds: Type} {R: Relation worlds} (d: Ensemble worlds): Prop :=
+  forall w1 w2, w1 <= w2 -> (d w1 <-> d w2).
+
+Class IdentityKripkeIntuitionisticModel (worlds: Type) {R: Relation worlds} : Prop := {
+  Korder_identity: forall m n: worlds, m <= n -> m = n
+}.
+
+Class NoBranchKripkeIntuitionisticModel (worlds: Type) {R: Relation worlds} : Prop := {
+  Korder_no_branch: forall m1 m2 n: worlds, n <= m1 -> n <= m2 -> m1 <= m2 \/ m2 <= m1
+}.
+
+Class BranchJoinKripkeIntuitionisticModel (worlds: Type) {R: Relation worlds} : Prop := {
+  Korder_branch_join: forall m1 m2 n: worlds, n <= m1 -> n <= m2 -> exists m, m1 <= m /\ m2 <= m
+}.
+
