PropositionalLogic/Semantics/Trivial.v
@@ -23,11 +23,19 @@ Definition falsep {model: Type}: Ensemble model := fun m => False.
 End Semantics.
 
 Class TrivialPropositionalSemantics (L: Language) {nL: NormalLanguage L} {pL: PropositionalLanguage L} (MD: Model) (SM: Semantics L MD): Type := {
+  denote_impp: forall x y, Same_set _ (denotation (x --> y)) (Semantics.impp (denotation x) (denotation y));
   denote_andp: forall x y, Same_set _ (denotation (x && y)) (Semantics.andp (denotation x) (denotation y));
   denote_orp: forall x y, Same_set _ (denotation (x || y)) (Semantics.orp (denotation x) (denotation y));
-  denote_impp: forall x y, Same_set _ (denotation (x --> y)) (Semantics.impp (denotation x) (denotation y));
   denote_falsep: Same_set _ (denotation FF) Semantics.falsep
 }.
+
+Lemma sat_impp {L: Language} {nL: NormalLanguage L} {pL: PropositionalLanguage L} {MD: Model} {SM: Semantics L MD} {tpSM: TrivialPropositionalSemantics L MD SM}: forall m x y, m |= x --> y <-> (m |= x -> m |= y).
+Proof.
+  intros; simpl.
+  unfold satisfies.
+  destruct (denote_impp x y).
+  split; auto; [apply H | apply H0].
+Qed.
 
 Lemma sat_andp {L: Language} {nL: NormalLanguage L} {pL: PropositionalLanguage L} {MD: Model} {SM: Semantics L MD} {tpSM: TrivialPropositionalSemantics L MD SM}: forall m x y, m |= x && y <-> (m |= x /\ m |= y).
 Proof.
@@ -42,14 +50,6 @@ Proof.
   intros; simpl.
   unfold satisfies.
   destruct (denote_orp x y).
-  split; auto; [apply H | apply H0].
-Qed.
-
-Lemma sat_impp {L: Language} {nL: NormalLanguage L} {pL: PropositionalLanguage L} {MD: Model} {SM: Semantics L MD} {tpSM: TrivialPropositionalSemantics L MD SM}: forall m x y, m |= x --> y <-> (m |= x -> m |= y).
-Proof.
-  intros; simpl.
-  unfold satisfies.
-  destruct (denote_impp x y).
   split; auto; [apply H | apply H0].
 Qed.
 
